define BExpr semantics

formal/Formal/Basic.lean
@@ -1,1 +1,32 @@
-def hello := "world"
+inductive BExpr where
+| True
+| False
+| If (ante : BExpr) (e1 : BExpr) (e2 : BExpr)
+
+inductive BExpr.Semantics : BExpr → BExpr → Prop where
+| IfTrue (t₂ t₃ : BExpr) : Semantics (If True t₂ t₃) t₂
+| IfFalse (t₂ t₃ : BExpr) : Semantics (If False t₂ t₃) t₃
+| IfCongr (t₁ t₁' t₂ t₃ : BExpr) :
+    Semantics t₁ t₁' → Semantics (If t₁ t₂ t₃) (If t₁' t₂ t₃)
+
+-- write using '\' + '~>'
+notation t₁ " ⤳ " t₂ => BExpr.Semantics t₁ t₂
+
+namespace BExpr
+
+abbrev tru := BExpr.True
+
+abbrev fls := BExpr.False
+
+notation "if_ " t₁ "then " t₂ "else " t₃ => BExpr.If t₁ t₂ t₃
+
+abbrev s := if_ tru then fls else fls
+
+abbrev t := if_ s then tru else tru
+
+abbrev u := if_ fls then tru else tru
+
+example : (if_ t then fls else fls) ⤳ (if_ u then fls else fls) := by
+  refine Semantics.IfCongr _ _ _ _ ?_
+  refine Semantics.IfCongr _ _ _ _ ?_
+  refine Semantics.IfTrue _ _
